theories/lang/cpp/specs/classy.v
@@ -16,6 +16,54 @@ Require Import iris.bi.bi.
 Require Import bedrock.prelude.bytestring_core.
 Require Import bedrock.lang.bi.only_provable.
 Require Import bedrock.lang.cpp.specs.spec_notations.
+Require Ltac2.Ltac2.
+
+Module Binder.
+  Import Ltac2.
+  Import Ltac2.Printf.
+  Import Ltac2.Constr.
+  Import Ltac2.Constr.Unsafe.
+
+  Ltac2 Type exn ::= [No].
+
+  Ltac2 to_bs (s : string) :=
+    let cons := constr:(@BS.String) in
+    let univs := match kind constr:(Byte.x00) with | Constructor _ univs => univs | _ => Control.throw No end in
+    let byte :=
+      match Option.get (Env.get (Env.path reference:(Byte.byte))) with
+      | Std.IndRef ind => ind
+      | _ => Control.throw No
+      end
+    in
+    let rec go i acc : constr :=
+      let i := Int.sub i 1 in
+      if Int.lt i 0 then acc else
+      let c := String.get s i in
+      let c := Char.to_int c in
+      let acc := make (App cons [|make (Constructor (Constr.Unsafe.constructor byte c) univs); acc|]) in
+      go i acc
+    in
+    go (String.length s) constr:(BS.EmptyString).
+
+  Ltac2 binder (p : Ltac1.t) :=
+    let p := Option.get (Ltac1.to_constr p) in
+    (* printf "%t" p; *)
+    let id := match Constr.Unsafe.kind p with
+    | Constr.Unsafe.Lambda b _ =>
+        (Option.default (@anon) (Constr.Binder.name b))
+    | _ => @anon
+    end in
+    refine (to_bs (Ident.to_string id)).
+End Binder.
+
+Class Binder {P : Type} (p : P) := binder : BS.t.
+Hint Opaque Binder : typeclass_instances.
+Ltac binder p :=
+  let f := ltac2:(p |- Binder.binder p) in
+  f p.
+#[global] Hint Extern 0 (Binder ?p) => binder p : typeclass_instances.
+
+#[global] Notation "'[binder' x ]" := (_ :> @Binder (forall x, True) (fun x => I)) (at level 0, x binder).
 
 Section with_prop.
   Context {PROP : bi} {spec_car : Type}.
@@ -23,7 +71,7 @@ Section with_prop.
   Class SpecGen : Type :=
     { add_pre : PROP -> spec_car -> spec_car
     ; add_post : PROP -> spec_car -> spec_car
-    ; add_with : forall {T : Type@{universes.Quant}}, (T -> spec_car) -> spec_car
+    ; add_with : forall {T : Type@{universes.Quant}}, (T -> spec_car) -> BS.t -> spec_car
     ; add_prepost (P : PROP) (S : spec_car) : spec_car :=
       add_pre P (add_post P S)
     ; add_require (P : Prop) : spec_car -> spec_car :=
@@ -40,7 +88,7 @@ Section with_prop.
   Class WithPost {RESULT : Type} : Type :=
     { post_car : Type
     ; start_post : post_car -> spec_car
-    ; post_with : forall T : Type@{universes.Quant}, (T -> post_car) -> post_car
+    ; post_with : forall T : Type@{universes.Quant}, (T -> post_car) -> BS.t -> post_car
     ; post_ret : RESULT -> PROP -> post_car
     }.
 
@@ -82,50 +130,70 @@ Declare Scope pre_spec_scope.
 Delimit Scope pre_spec_scope with pre_spec.
 
 Notation "'\with' x .. y X" :=
-  (add_with (fun x => .. (add_with (fun y => X%pre_spec)) ..)).
+  (add_with (fun x => .. (add_with (fun y => X%pre_spec) [binder y]) ..) [binder x]) (only parsing).
+Notation "'\with' x .. y X" :=
+  (add_with (fun x => .. (add_with (fun y => X%pre_spec) _) ..) _) (only printing).
 
 Notation "'\prepost' pp X" := (add_prepost pp%I X%pre_spec).
 
 Notation "'\prepost{' x .. y '}' pp X" :=
-  (add_with (fun x => .. (add_with (fun y => add_prepost pp%I X%pre_spec)) ..)).
+  (add_with (fun x => .. (add_with (fun y => add_prepost pp%I X%pre_spec) [binder y]) ..) [binder x]) (only parsing).
+Notation "'\prepost{' x .. y '}' pp X" :=
+  (add_with (fun x => .. (add_with (fun y => add_prepost pp%I X%pre_spec) _) ..) _) (only printing).
 
 Notation "'\let' x ':=' e X" := (let_pre_spec (let x := e in X%pre_spec)).
 
 Notation "'\let{' x .. y '}' z ':=' e X" :=
-  (add_with (fun x => .. (add_with (fun y => let_pre_spec (let z := e in X%pre_spec))) ..)).
+  (add_with (fun x => .. (add_with (fun y => let_pre_spec (let z := e in X%pre_spec)) [binder y]) ..) [binder x]) (only parsing).
+Notation "'\let{' x .. y '}' z ':=' e X" :=
+  (add_with (fun x => .. (add_with (fun y => let_pre_spec (let z := e in X%pre_spec)) _) ..) _) (only printing).
 
 Notation "'\arg' nm v X" := (add_named_arg nm%bs v X%pre_spec).
 
 Notation "'\arg{' x .. y } nm v X" :=
-  (add_with (fun x => .. (add_with (fun y => add_named_arg nm%bs v X%pre_spec)) ..)).
+  (add_with (fun x => .. (add_with (fun y => add_named_arg nm%bs v X%pre_spec) [binder y]) ..) [binder x]) (only parsing).
+Notation "'\arg{' x .. y } nm v X" :=
+  (add_with (fun x => .. (add_with (fun y => add_named_arg nm%bs v X%pre_spec) _) ..) _) (only printing).
 
 Notation "'\args' v X" := (add_args v X%pre_spec).
 
 Notation "'\args{' x .. y } v X" :=
-  (add_with (fun x => .. (add_with (fun y => add_args v X%pre_spec)) ..)).
+  (add_with (fun x => .. (add_with (fun y => add_args v X%pre_spec) [binder y]) ..) [binder x]) (only parsing).
+Notation "'\args{' x .. y } v X" :=
+  (add_with (fun x => .. (add_with (fun y => add_args v X%pre_spec) _) ..) _) (only printing).
 
 Notation "'\require' pre X" := (add_require pre X%pre_spec).
 
 Notation "'\require{' x .. y } pre X" :=
-  (add_with (fun x => .. (add_with (fun y => add_require pre X%pre_spec)) ..)).
+  (add_with (fun x => .. (add_with (fun y => add_require pre X%pre_spec) [binder y]) ..) [binder x]) (only parsing).
+Notation "'\require{' x .. y } pre X" :=
+  (add_with (fun x => .. (add_with (fun y => add_require pre X%pre_spec) _) ..) _) (only printing).
 
 Notation "'\persist' pre X" := (add_persist pre%I X%pre_spec).
 
 Notation "'\persist{' x .. y } pre X" :=
-  (add_with (fun x => .. (add_with (fun y => add_persist pre%I X%pre_spec)) ..)).
+  (add_with (fun x => .. (add_with (fun y => add_persist pre%I X%pre_spec) [binder y]) ..) [binder x]) (only parsing).
+Notation "'\persist{' x .. y } pre X" :=
+  (add_with (fun x => .. (add_with (fun y => add_persist pre%I X%pre_spec) _) ..) _) (only printing).
 
 Notation "'\pre' pre X" := (add_pre pre%I X%pre_spec).
 
 Notation "'\pre{' x .. y '}' pp X" :=
-  (add_with (fun x => .. (add_with (fun y => add_pre pp%I X%pre_spec)) ..)).
+  (add_with (fun x => .. (add_with (fun y => add_pre pp%I X%pre_spec) [binder y]) ..) [binder x]) (only parsing).
+Notation "'\pre{' x .. y '}' pp X" :=
+  (add_with (fun x => .. (add_with (fun y => add_pre pp%I X%pre_spec) _) ..) _) (only printing).
 
 Notation "'\post*{' x .. y '}' post X" :=
-  (add_with (fun x => .. (add_with (fun y => add_post post%I X%pre_spec)) ..)).
+  (add_with (fun x => .. (add_with (fun y => add_post post%I X%pre_spec) [binder y]) ..) [binder x]) (only parsing).
+Notation "'\post*{' x .. y '}' post X" :=
+  (add_with (fun x => .. (add_with (fun y => add_post post%I X%pre_spec) _) ..) _) (only printing).
 
 Notation "'\post*' post X" := (add_post post%I X%pre_spec).
 
 Notation "'\post' { x .. y } [ r ] post" :=
-  (start_post (post_with (fun x => .. (post_with (fun y => post_ret r post%I)) ..))).
+  (start_post (post_with (fun x => .. (post_with (fun y => post_ret r post%I) [binder y]) ..) [binder x])) (only parsing).
+Notation "'\post' { x .. y } [ r ] post" :=
+  (start_post (post_with (fun x => .. (post_with (fun y => post_ret r post%I) _) ..) _)) (only printing).
 
 Notation "'\post' [ r ] post" :=
   (start_post (post_ret r post%I)).
